Benchmark/Generated/Polaris/BondingCurve/Tasks/sell_preserves_reserve_ratio_zero.lean
@@ -8,13 +8,16 @@ open Verity.EVM.Uint256
 
 theorem sell_preserves_reserve_ratio_zero_task
     (bcTokenAmount computedNewVirtualBalance : Uint256) (s : ContractState)
-    (hNetAmountNonZero :
-      sub bcTokenAmount (div (mul bcTokenAmount (feePercentageOf s)) decimalPrecision) != 0)
+    (hNetAmountNonZero : sellNetBurnAmount bcTokenAmount s != 0)
     (hComputedNewVirtual :
-      computedNewVirtualBalance =
-        curveBalance
-          (sub (add (floorSupplyOf s) (totalSupplyOf s))
-            (sub bcTokenAmount (div (mul bcTokenAmount (feePercentageOf s)) decimalPrecision)))) :
+      trustedCurveHelperOutput (sellVirtualSupplyAfter bcTokenAmount s)
+        computedNewVirtualBalance)
+    (hOldSupplyNoOverflow :
+      (floorSupplyOf s).val + (totalSupplyOf s).val < Verity.Core.Uint256.modulus)
+    (hNetLeOldSupply : sellNetBurnAmount bcTokenAmount s <= virtualSupplyOf s)
+    (hNetLeTotalSupply : sellNetBurnAmount bcTokenAmount s <= totalSupplyOf s)
+    (hNetValLeTotalSupply :
+      (sellNetBurnAmount bcTokenAmount s).val <= (totalSupplyOf s).val) :
     let s' := ((BaseBondingCurve.sell bcTokenAmount computedNewVirtualBalance).run s).snd
     sell_preserves_reserve_ratio_zero_spec s s' := by
   exact ?_
